

3.5

$$1 - \tilde{\Psi}(k) = \frac{1}{\sqrt{2\pi}} \int_{\mathbb{R}} dx e^{-ikx} \Psi(x)$$

$$\Psi(x) = \frac{1}{\sqrt{2\pi}} \int_{\mathbb{R}} dk e^{+ikx} \tilde{\Psi}(k)$$

A) FOURIER TRANSFORM OF

$$\Psi(x) = (\pi\omega_0^2)^{-\frac{1}{4}} \exp\left(i p_0 \frac{x}{\hbar} - \frac{(x-x_0)^2}{2\omega_0^2}\right)$$

$$x_0, p_0, \omega_0 \in \mathbb{R}$$

$$1 \rightarrow \tilde{\Psi}(k) = \frac{1}{\sqrt{2\pi}} \int_{\mathbb{R}} dx \exp(-ikx) \exp\left(i p_0 \frac{x}{\hbar} - \frac{(x-x_0)^2}{2\omega_0^2}\right)$$

$$\sqrt[4]{\pi\omega_0^2}$$

$$= \frac{1}{\sqrt{2\pi} \cdot \sqrt[4]{\pi\omega_0^2}} \int_{\mathbb{R}} dx \exp(-ikx) \exp\left(\frac{i p_0 x}{\hbar}\right) \exp\left(-\frac{(x-x_0)^2}{2\omega_0^2}\right)$$

MULTIPLY BY : $\rightarrow \frac{\exp(-ikx_0)}{\exp(-ikx_0)} \cdot \frac{\exp(i p_0 x_0 / \hbar)}{\exp(i p_0 x_0 / \hbar)}$

$$= \frac{\text{EXP}(-ikx_0) \cdot \text{EXP}(ip_0/\hbar x_0)}{\sqrt{2\pi} \sqrt[4]{\pi \omega_0^2}} \int_{\mathbb{R}} dx \text{EXP}(ik(x-x_0)) \text{EXP}\left(\frac{ip_0}{\hbar}(x-x_0)\right) \text{EXP}\left(-\frac{(x-x_0)^2}{2\omega_0^2}\right)$$

CALL IT W FOR NOW

$\rightarrow x' = x - x_0 \quad dx' = dx$

$$= W \int_{\mathbb{R}} dx' \text{EXP}(ikx') \text{EXP}\left(\frac{ip_0}{\hbar}x'\right) \text{EXP}\left(-\frac{x'^2}{2\omega_0^2}\right)$$

$$= W \int_{\mathbb{R}} dx' \text{EXP}\left(-\underbrace{\frac{1}{2\omega_0^2}}_{\hookrightarrow a} x'^2 + \underbrace{i\left(k + \frac{p_0}{\hbar}\right)}_{\hookrightarrow b} x'\right)$$

\hookrightarrow KNOWN GAUSSIAN INTEGRAL IN THE FORM:

$$\int_{-\infty}^{+\infty} e^{-ax^2+bx} dx = e^{\frac{b^2}{4a}} \sqrt{\frac{\pi}{a}}$$

$$= W \text{EXP}\left(i^2 \frac{(k + p_0/\hbar)^2}{2\omega_0^2}\right) \sqrt{2\pi\omega_0^2}$$

$i^2 \rightarrow -1$

$$= \frac{\text{EXP}(-ikx_0) \text{EXP}\left(i\frac{p_0}{\hbar}x_0\right) \text{EXP}\left(-\frac{\omega_0^2}{2}\left(k + \frac{p_0}{\hbar}\right)^2\right) \sqrt{2\pi\omega_0^2}}{\sqrt{2\pi} \sqrt[4]{\pi \omega_0^2}}$$

$$= \text{EXP} \left(i \left(\frac{p_0}{\hbar} - k \right) x_0 - \frac{\omega_0^2}{2} \left(k + \frac{p_0}{\hbar} \right)^2 \right) \frac{\omega_0}{\sqrt[4]{\pi \omega_0^2}}$$

$$\Rightarrow \tilde{\psi}(k) = e^{i \left(\frac{p_0}{\hbar} - k \right) x_0} \cdot e^{-\frac{\omega_0^2}{2} \left(k + \frac{p_0}{\hbar} \right)^2} \cdot \frac{\omega_0}{\sqrt[4]{\pi \omega_0^2}}$$

VERIFY BY NORMALIZING:

$$\int_{\mathbb{R}} dk |\psi(k)|^2 = 1 \quad \Rightarrow \quad \int_{\mathbb{R}} \psi(k) \cdot \psi^*(k) dk = 1$$

$$\Rightarrow \int_{\mathbb{R}} e^{i \left(\frac{p_0}{\hbar} - k \right) x_0} \cdot e^{-\frac{\omega_0^2}{2} \left(k + \frac{p_0}{\hbar} \right)^2} \cdot \frac{\omega_0}{\sqrt[4]{\pi \omega_0^2}} \cdot e^{-i \left(\frac{p_0}{\hbar} - k \right) x_0} \cdot e^{-\frac{\omega_0^2}{2} \left(k + \frac{p_0}{\hbar} \right)^2} \cdot \frac{\omega_0}{\sqrt[4]{\pi \omega_0^2}} dk$$

$e^0 = 1$

$$= \frac{\omega_0}{\sqrt{\pi}} \int_{\mathbb{R}} e^{-\omega_0^2 \left(k + \frac{p_0}{\hbar} \right)^2} dk$$

GAUSSIAN: $\int_{\mathbb{R}} e^{-a(x+b)^2} = \sqrt{\frac{\pi}{a}}$

$$= \frac{\cancel{\omega_0}}{\cancel{\sqrt{\pi}}} \sqrt{\frac{\pi}{\omega_0^2}} = 1 \quad \checkmark \checkmark$$

B

$$\text{show } \langle \hat{x} \rangle = \langle \Psi | \hat{x} \Psi \rangle = x_0$$

$$\langle \hat{p} \rangle = \langle \Psi | \hat{p} \Psi \rangle = p_0$$

$$\text{w 1m } (\hat{p} \Psi)(x) = -i\hbar \frac{d}{dx} \Psi(x)$$

$$(\hat{x} \Psi)(x) = x \Psi(x) \quad \text{Ans}$$

$$\langle \Psi | \phi \rangle = \int_{\mathbb{R}} \overline{\Psi(x)} \phi(x) dx$$

$$(1) \quad \langle \Psi(x) | (\hat{x} \Psi)(x) \rangle = \int_{\mathbb{R}} \overline{\Psi(x)} \cdot (\hat{x} \Psi)(x) dx$$

$$= \int_{\mathbb{R}} \overline{\Psi(x)} \Psi(x) x dx$$

$$= \int_{\mathbb{R}} (\pi \omega_0^2)^{-\frac{1}{4}} \cdot \exp(-i p_0 \frac{x}{\hbar}) \exp(-\frac{(x-x_0)^2}{2\omega_0^2}) dx$$

$$\updownarrow \exp(0) = 1$$

$$(\pi \omega_0^2)^{-\frac{1}{4}} \cdot \exp(-i p_0 \frac{x}{\hbar}) \exp(-\frac{(x-x_0)^2}{2\omega_0^2}) \cdot x$$

$$= \frac{1}{\sqrt{\pi \omega_0^2}} \int_{\mathbb{R}} \exp(-\frac{2(x-x_0)^2}{2\omega_0^2}) x dx$$

$$X' = X - X_0 \rightarrow X = X' + X_0$$

$$dx = dx'$$

$$\Rightarrow = \frac{1}{\sqrt{\pi \omega_0^2}} \int_{\mathbb{R}} \exp\left(-\frac{1}{\omega_0^2} (X')^2\right) (X' + X_0) dx$$

$$= \frac{1}{\sqrt{\pi \omega_0^2}} \left(\underbrace{\int_{-\infty}^{\infty} e^{-\frac{1}{\omega_0^2} (X')^2} (X') dx}_{\substack{\text{EVEN F} \\ \downarrow \\ \text{ODD F over} \\ \text{A } \pm \text{ interval} = 0}} + X_0 \underbrace{\int_{-\infty}^{\infty} e^{-\frac{1}{\omega_0^2} (X')^2} dx}_{\text{GAUSSIAN IN THE FORM}} \right)$$

$$\int_{-\infty}^{\infty} e^{-a x^2} dx = \sqrt{\frac{\pi}{a}}$$

$$= \omega_0 \sqrt{\pi}$$

$$\Rightarrow \langle \hat{X} \rangle = \frac{X_0 \omega_0 \sqrt{\pi}}{\omega_0 \sqrt{\pi}} = X_0$$

$$(2) \quad \langle \hat{p} \rangle = \langle \psi(x) | (\hat{p} \psi)(x) \rangle$$

$$= \int_{\mathbb{R}} dx \overline{\psi(x)} (\hat{p} \psi)(x) = \int_{\mathbb{R}} dx \overline{\psi(x)} (-i\hbar \frac{d}{dx} \psi(x))$$

$$\bullet \quad \frac{d}{dx} \psi(x) = \frac{d}{dx} (\pi \omega_0^2)^{-\frac{1}{4}} \cdot \text{EXP}\left(i \rho_0 \frac{x}{\hbar}\right) \text{EXP}\left(-\frac{(x-x_0)^2}{2\omega_0^2}\right)$$

$$= (\pi \omega_0^2)^{-\frac{1}{4}} \frac{d}{dx} \text{EXP}\left(i \rho_0 \frac{x}{\hbar} - \frac{(x^2 + x_0^2 - 2x_0 x)}{2\omega_0^2}\right)$$

$$= (\pi \omega_0^2)^{-\frac{1}{4}} \frac{d}{dx} \text{EXP}\left(\frac{2\omega_0^2 i \rho_0 x - \hbar x^2 - \hbar x_0^2 + 2x_0 \hbar x}{2\omega_0^2 \hbar}\right)$$

$$= (\pi \omega_0^2)^{-\frac{1}{4}} \frac{d}{dx} \text{EXP}\left(-\frac{1}{2\omega_0^2} x^2 + \left(\frac{\omega_0^2 i \rho_0 + x_0 \hbar}{\omega_0^2 \hbar}\right) x - \frac{x_0^2}{2\omega_0^2}\right)$$

$$= (\pi \omega_0^2)^{-\frac{1}{4}} \text{EXP}\left(i \rho_0 \frac{x}{\hbar}\right) \text{EXP}\left(-\frac{(x-x_0)^2}{2\omega_0^2}\right) \left(-\frac{x}{\omega_0^2} + \frac{i\omega_0^2 \rho_0 + x_0 \hbar}{\omega_0^2 \hbar}\right)$$

$$\Rightarrow \langle \hat{p} \rangle = \int_{\mathbb{R}} dx (\pi \omega_0^2)^{-\frac{1}{4}} \cdot \text{EXP}\left(-i \rho_0 \frac{x}{\hbar}\right) \text{EXP}\left(-\frac{(x-x_0)^2}{2\omega_0^2}\right)$$

$$(-i\hbar) (\pi \omega_0^2)^{-\frac{1}{4}} \text{EXP}\left(i \rho_0 \frac{x}{\hbar}\right) \text{EXP}\left(-\frac{(x-x_0)^2}{2\omega_0^2}\right) \left(-\frac{x}{\omega_0^2} + \frac{i\omega_0^2 \rho_0 + x_0 \hbar}{\omega_0^2 \hbar}\right)$$

$$= (\pi \omega_0^2)^{-\frac{1}{2}} (-i\hbar) \int_{\mathbb{R}} dx \left(\exp\left(-\frac{(x-x_0)^2}{\omega_0^2}\right) \left(-\frac{x}{\omega_0^2} + \frac{i\omega_0^2 p_0 + x_0 \hbar}{\omega_0^2 \hbar}\right) \right)$$

$$= (\pi \omega_0^2)^{-\frac{1}{2}} (-i\hbar) \left(\int_{\mathbb{R}} dx \exp\left(-\frac{(x-x_0)^2}{\omega_0^2}\right) \left(-\frac{x}{\omega_0^2}\right) + \int_{\mathbb{R}} dx \exp\left(-\frac{(x-x_0)^2}{\omega_0^2}\right) \left(\frac{i\omega_0^2 p_0 + x_0 \hbar}{\omega_0^2 \hbar}\right) \right)$$

$x' = x - x_0 \rightarrow x = x' + x_0$
 $\rightarrow dx = dx'$

$$= \int_{\mathbb{R}} dx' \exp\left(-\frac{1}{\omega_0^2} x'^2\right) \left(-\frac{x'}{\omega_0} - \frac{x_0}{\omega_0}\right)$$

LIKE BEFORE

$$= -\frac{1}{\omega_0^2} \int_{\mathbb{R}} dx' \exp\left(-\frac{1}{\omega_0^2} x'^2\right) \underbrace{x'}_{\text{ODD}} - \frac{x_0}{\omega_0} \int_{\mathbb{R}} dx' e^{-\frac{1}{\omega_0^2} x'^2}$$

EVEN $\rightarrow \int_{-\infty}^{\infty} \text{ODD f(x)} = 0$

GAUSSIAN:

$$\int_{-\infty}^{\infty} dx e^{-\alpha x^2} = \sqrt{\frac{\pi}{\alpha}}$$

$$= \sqrt{\pi \omega_0^2}$$

$$= -\frac{x_0 \omega_0 \sqrt{\pi}}{\omega_0^2} = -\frac{\sqrt{\pi}}{\omega_0} x_0$$

$$= (\pi \omega_0^2)^{-\frac{1}{2}} (-i\hbar) \left(-\sqrt{\pi} x_0 + \int_{\mathbb{R}} dx' \exp\left(-\frac{(x')^2}{\omega_0^2}\right) \left(\frac{i\omega_0^2 p_0 + x_0 \hbar}{\omega_0^2 \hbar}\right) \right)$$

$$= (\pi \omega_0^2)^{-\frac{1}{2}} (-i\hbar) \left(-\frac{\sqrt{\pi} x_0}{\omega_0} + \left(\frac{i\omega_0^2 \rho_0 + x_0 \hbar}{\omega_0^2 \hbar} \right) \right) \int_{\mathbb{R}} dx' \exp\left(-\frac{1}{\omega_0^2} x'^2\right)$$

$= \cancel{\omega_0} \sqrt{\pi}$

$$= \frac{(-i\hbar)}{\omega_0 \sqrt{\pi}} \left(-\frac{\cancel{\sqrt{\pi}} x_0}{\omega_0} + \frac{\cancel{\sqrt{\pi}} i\omega_0^2 \rho_0 + \cancel{\sqrt{\pi}} x_0 \hbar}{\omega_0 \hbar} \right)$$

$$= \left(\frac{-i\hbar}{\omega_0} \right) \left(\frac{-\cancel{\hbar} x_0 + i\omega_0^2 \rho_0 + \cancel{x_0} \hbar}{\omega_0 \cancel{\hbar}} \right)$$

$$= \cancel{\omega_0} \frac{-i\omega_0^2}{\omega_0} \rho_0 = \rho_0$$

$$c) \quad \phi(x) = (\pi \omega_0^2)^{-\frac{1}{4}} e^{i p_1 \frac{x}{\hbar} - (x - x_1)^2 / (2 \omega_0^2)}$$

$$= (\pi \omega_0^2)^{-\frac{1}{4}} \exp\left(i p_1 \frac{x}{\hbar}\right) \exp\left(-\frac{(x - x_1)^2}{2 \omega_0^2}\right)$$

$$\text{CALCULATE } \langle \psi | \phi \rangle = \int_{\mathbb{R}} \bar{\psi} \phi dx$$

$$\left(-\frac{(x - x_1)^2 + (x - x_0)^2}{2 \omega_0^2} \right)$$

⇓

$$= (\pi \omega_0^2)^{-\frac{1}{2}} \int_{\mathbb{R}} dx \exp\left(i \frac{x}{\hbar} (p_1 - p_0)\right) \exp\left(-\frac{2x^2 - 2(x_0 + x_1)x + x_1^2 + x_0^2}{2 \omega_0^2}\right)$$

↓

↙

$$\frac{2i \omega_0^2 (p_1 - p_0) x - 2\hbar x^2 + 2\hbar (x_0 + x_1)x - (x_1^2 + x_0^2)\hbar}{2\hbar \omega_0^2}$$

$$= (\pi \omega_0^2)^{-\frac{1}{2}} \int_{\mathbb{R}} dx \exp\left(-\frac{2\hbar x^2 + 2\left[i \omega_0^2 (p_1 - p_0) + \hbar (x_0 + x_1)\right]x - (x_1^2 + x_0^2)\hbar}{2\hbar \omega_0^2}\right)$$

$$= (\pi \omega_0^2)^{-\frac{1}{2}} \exp\left(-\frac{(x_1^2 + x_0^2)}{2 \omega_0^2}\right) \int_{\mathbb{R}} dx \exp\left[-\frac{1}{\omega_0^2} x^2 + \frac{i \omega_0^2 (p_1 - p_0) + \hbar (x_0 + x_1)}{\hbar \omega_0^2} x\right]$$

GAUSSIAN or THE FORM $\int_{-\infty}^{\infty} e^{-ax^2 + bx} dx = e^{\frac{b^2}{4a}} \sqrt{\frac{\pi}{a}} \rightarrow$

$$\rightarrow \left[\text{EXP} \left(\frac{(i\omega_0^2(p_1 - p_0) + \hbar(x_1 + x_0))^2}{\hbar^2 \omega_0^4} \cdot \frac{\cancel{\omega_0^2}}{4} \right) \omega_0 \sqrt{\pi} \right]$$

$$= \frac{\cancel{\omega_0 \sqrt{\pi}}}{\omega_0 \sqrt{\pi}} \text{EXP} \left(-\frac{(x_1^2 + x_0^2)}{2\omega_0^2} + \frac{1}{4\hbar^2 \omega_0^2} \underbrace{(i\omega_0^2(p_1 - p_0) + \hbar(x_1 + x_0))^2}_{\text{expanded below}} \right)$$

$$\rightarrow -\omega_0^4(p_1 - p_0)^2 + \hbar^2(x_1 + x_0)^2 + 2i\hbar\omega_0^2(p_1 - p_0)(x_1 + x_0)$$

$$= \text{EXP} \left[\frac{-2\hbar^2 x_1^2 - 2\hbar^2 x_0^2 - \omega_0^4(p_1 - p_0)^2 + \hbar^2(x_1 + x_0)^2 + 2i\hbar\omega_0^2(p_1 - p_0)(x_1 + x_0)}{4\omega_0^2 \hbar^2} \right]$$

$\hbar^2(2x_1^2 + 2x_0^2 - x_1^2 - x_0^2 - 2x_0x_1) = \hbar^2(x_1^2 + x_0^2 - 2x_0x_1) = \hbar^2(x_1 - x_0)^2$

$$= \text{EXP} \left[\frac{2\hbar^2 x_1^2 + 2\hbar^2 x_0^2 - \hbar^2(x_1 + x_0)^2 + \omega_0^4(p_1 - p_0)^2 - 2i\hbar\omega_0^2(p_1 - p_0)(x_1 + x_0)}{4\omega_0^2 \hbar^2} \right]$$

$$= \text{EXP} \left[\frac{\hbar^2(x_1 - x_0)^2 + \omega_0^4(p_1 - p_0)^2 - 2i\hbar\omega_0^2(p_1 - p_0)(x_1 + x_0)}{4\omega_0^2 \hbar^2} \right]$$

D

WE KNOW THE OPERATIONS \hat{x} , \hat{p} ARE SELF-ADJOINT:

THAT IS:
$$\begin{cases} \hat{x} = \hat{x}^\dagger \\ \hat{p} = \hat{p}^\dagger \end{cases}$$

TO PROVE THIS:

FOR \hat{x} : POSITION IS SUCH THAT

$$\langle \phi | \hat{x} \psi \rangle = \langle \hat{x}^\dagger \phi | \psi \rangle$$

LHS:

$$\langle \phi | \hat{x} \psi \rangle = \int \phi^* x \psi dx$$

RHS:

$$\langle \hat{x}^\dagger \phi | \psi \rangle = \int (\hat{x}^\dagger \phi)^* \psi$$

$$= \int (\hat{x}^\dagger)^* \phi^* \psi dx$$

EIGENV.
OF $\hat{x} \rightarrow \hat{x}^\dagger$
ARE REAL:
 $x^* = x$

$$= \int x \phi^* \psi dx$$

$$\Rightarrow \hat{x} = \hat{x}^\dagger$$

For \hat{p} :

$$\langle \phi | \hat{p} \psi \rangle = \langle \hat{p}^\dagger \phi | \psi \rangle$$

$$\text{LHS: } \langle \phi | \hat{p} \psi \rangle = \int \phi^* (-i\hbar) \frac{\partial \psi}{\partial x} dx$$

$$\text{RHS: } \langle \hat{p}^\dagger \phi | \psi \rangle = \int (\hat{p}^\dagger \phi)^* \psi dx$$

$$= \int \left(i\hbar \frac{\partial \phi^*}{\partial x} \right) \psi dx$$

$$= i\hbar \int \frac{\partial \phi^*}{\partial x} \psi dx$$

by parts:

$$= i\hbar \left(\left[\phi^* \psi \right]_{-\infty}^{\infty} - \int \phi^* \frac{\partial \psi}{\partial x} dx \right)$$

IGNORE BOUND. COND.

$$= \int \phi^* (-i\hbar) \frac{\partial \psi}{\partial x} dx \quad \Leftrightarrow \quad \hat{p} = \hat{p}^\dagger$$

THE, WHEN DEALING WITH COMPOSITE VECS:

$$\bullet \hat{x} \hat{p} + \hat{p} \hat{x} \xrightarrow{\text{ADJOINT}} (\hat{x} \hat{p} + \hat{p} \hat{x})^\dagger = (\hat{x} \hat{p})^\dagger + (\hat{p} \hat{x})^\dagger =$$

$$= \hat{p}^\dagger \hat{x}^\dagger + \hat{x}^\dagger \hat{p}^\dagger \quad \text{BUT} \quad \hat{x} = \hat{x}^\dagger, \hat{p} = \hat{p}^\dagger$$

$$\Rightarrow = \hat{p} \hat{x} + \hat{x} \hat{p}$$

↓
WITH A TEST FUNCTION:

$$(\hat{p} \hat{x} + \hat{x} \hat{p}) \psi(x) = -i\hbar \frac{\partial}{\partial x} (x \cdot \psi(x)) + x (-i\hbar) \frac{\partial}{\partial x} \psi(x)$$

$$= -i\hbar \left(\psi(x) + x \frac{\partial}{\partial x} \psi(x) + x \frac{\partial}{\partial x} \psi(x) \right)$$

$$= -i\hbar \left(\psi(x) + 2x \frac{\partial}{\partial x} \psi(x) \right)$$

$$\Rightarrow \hat{p} \hat{x} + \hat{x} \hat{p} = -i\hbar \left(1 + 2x \frac{\partial}{\partial x} \right)$$

$$\bullet \hat{x} \hat{p}^m \hat{x} \xrightarrow{\text{ADJOINT}} (\hat{x} \hat{p}^m \hat{x})^\dagger =$$

$$= (\hat{p}^m \hat{x})^\dagger \hat{x}^\dagger = \hat{x}^\dagger (\hat{p}^m)^\dagger \hat{x}^\dagger$$

ASSUME $m = 3$: $\hat{p}^3 = (\hat{p} \hat{p} \hat{p})^\dagger = \hat{p}^\dagger \hat{p}^\dagger \hat{p}^\dagger = \hat{p} \hat{p} \hat{p} = \hat{p}^3$

\Rightarrow ADJOINT D ITSELF: $(\hat{x} \hat{p}_m \hat{x})^\dagger = \hat{x} \hat{p}_m \hat{x}$

$= x \left(\frac{\partial^m}{\partial x^m} x \right)$

↓
WI TH TEST FUNCTION:

$(\hat{x} \hat{p}_m \hat{x}) \psi(x) = -i\hbar x \frac{\partial^m}{\partial x^m} (x \psi(x))$

↓
LEIBNIZ RULE:

$(fg)^{(m)} = \sum_{k=0}^m \binom{m}{k} f^{(m-k)} g^{(k)}$

$\frac{\partial^{m-1}}{\partial x^{m-1}} \left(\frac{\partial}{\partial x} (x \psi(x)) \right) = \frac{\partial^{m-1}}{\partial x^{m-1}} \left(\psi(x) + x \frac{\partial}{\partial x} \psi(x) \right)$

$= \frac{\partial^{m-2}}{\partial x^{m-2}} \left(\frac{\partial}{\partial x} \psi(x) + \frac{\partial}{\partial x} \psi(x) + x \frac{\partial^2}{\partial x^2} \psi(x) \right)$

$= \frac{\partial^{m-3}}{\partial x^{m-3}} \left(2 \frac{\partial^2}{\partial x^2} \psi(x) + \frac{\partial^2}{\partial x^2} \psi(x) + x \frac{\partial^3}{\partial x^3} \psi(x) \right)$

$= \left[(m) \frac{\partial^{m-1}}{\partial x^{m-1}} \psi(x) + x \frac{\partial^m}{\partial x^m} \psi(x) \right]$

$$\Rightarrow (\hat{x} \hat{p}^m \hat{x}) = -i\hbar (m \partial_{x^{m-1}} + x \partial_x)$$

$$\bullet (\hat{x} \hat{p})^m = \hat{x}^m \hat{p}^m \longrightarrow (\hat{x}^m \hat{p}^m)^\dagger \longrightarrow \hat{p}^m \hat{x}^m$$

↓ WITH TEST FUNCTION:

$$(\hat{p}^m \hat{x}^m) \psi(x) = -i\hbar \frac{\partial^m}{\partial x^m} (x^m \psi(x))$$

$$= \frac{\partial^{m-1}}{\partial x^{m-1}} \left(m x^{m-1} \psi(x) + x^m \frac{\partial}{\partial x} \psi(x) \right)$$

$$= \frac{\partial^{m-2}}{\partial x^{m-2}} \left(m \left((m-1) x^{m-2} \psi(x) + x^{m-1} \frac{\partial}{\partial x} \psi(x) \right) + m x^{m-1} \frac{\partial}{\partial x} \psi(x) + x^m \frac{\partial^2}{\partial x^2} \psi(x) \right)$$

$$= \partial_x^{m-2} \left(m(m-1) x^{m-2} \psi + m x^{m-1} \partial_x \psi + m x^{m-1} \partial_x \psi + x^m \partial_x^2 \psi \right)$$

$$\longrightarrow m! x^m \psi + 2m x^{m-1} \frac{\partial}{\partial x} \psi + x^m \frac{\partial^2}{\partial x^2} \psi$$

$$\Rightarrow (\hat{p} \hat{x})^m = \left(m! x^m + 2m x^{m-1} \partial_x + x^m \partial_x^2 \right)$$

e] COMPUTE VARIANCE FOR $\psi(x)$

- VARIANCE OF \hat{X} :

$$\Delta \hat{X} = \sqrt{\langle (\hat{X} - \langle \hat{X} \rangle)^2 \rangle}$$

FOR $\langle \hat{X} \rangle = \langle \psi | \hat{X} | \psi \rangle =$ WE FOUND IT BEFORE EQUAL TO x_0 :

$$\Delta \hat{X} = \sqrt{\langle (\hat{X} - x_0)^2 \rangle}$$

$$\langle (\hat{X} - x_0)^2 \rangle = \langle \psi | (\hat{X} - x_0)^2 | \psi \rangle$$

$$= \int_{\mathbb{R}} \bar{\psi} \cdot (\hat{X} - x_0)^2 \psi \, dx$$

$$= \int_{\mathbb{R}} \bar{\psi} (\hat{X}^2 + x_0^2 - 2x_0 \hat{X}) \psi$$

$$= \int_{\mathbb{R}} \bar{\psi} (x^2 + x_0^2 - 2x x_0) \psi$$

$\psi \cdot \bar{\psi} =$ FORM BEFORE;

$$= \frac{1}{\sqrt{\pi \omega_0^2}} \int_{\mathbb{R}} \exp\left(-\frac{2(x-x_0)^2}{2\omega_0^2}\right) (x-x_0)^2 dx$$

$$(x-x_0) = x' \quad dx = dx'$$

$$\Rightarrow \frac{1}{\sqrt{\pi \omega_0^2}} \int_{\mathbb{R}} \exp\left(-\frac{1}{\omega_0^2} x'^2\right) x'^2 dx'$$

Solve before by ans:

$$\Rightarrow = \frac{1}{\sqrt{\pi \omega_0^2}} \frac{\sqrt{\pi \omega_0^6}}{2} = \frac{1}{2} \frac{\omega_0^3}{\omega_0} = \frac{1}{2} \omega_0^2$$

$$\Rightarrow \Delta \hat{x} = \sqrt{\frac{\omega_0^2}{2}} = \frac{|\omega_0|}{\sqrt{2}}$$

• VARIANCE OF \hat{p} :

$$\Delta \hat{p} = \sqrt{\langle (\hat{p} - \underbrace{\langle \hat{p} \rangle}_{p_0})^2 \rangle} = \sqrt{\langle (\hat{p} - p_0)^2 \rangle}$$

$$\langle (\hat{p} - p_0)^2 \rangle = \langle \psi | (\hat{p} - p_0)^2 \psi \rangle$$

$$= \int_{\mathbb{R}} \bar{\psi} \cdot (\hat{p} - p_0)^2 \psi dx$$

$$= \int_{\mathbb{R}} \bar{\Psi} \left(\hat{p}^2 + p_0^2 - 2p_0 \hat{p} \right) \Psi \, dx$$

INTEGRATING BY PARTS AGAIN, WE FIND THAT

$$\langle (\hat{p} - p_0)^2 \rangle = \frac{\hbar^2}{2\omega_0^2}$$

$$\Rightarrow \Delta \hat{p} = \frac{\hbar}{|\omega_0| \sqrt{2}}$$

6)

$$\hat{H} = \frac{1}{2m} \hat{p}^2 = -\frac{\hbar^2}{2m} \frac{\partial^2}{\partial x^2}$$

SOLVE TIME DEPENDENT SCHRÖDINGER EQUATION:

$$i\hbar \frac{d}{dt} \psi(x) = \hat{H} \psi(x) \quad , \quad \psi_0(x) = \psi(x) \quad \left[\text{IN A} \right]$$